---
layout: page
title: 2021-09-16
parent: Notes
has_children: false
---

## Triangulated categories

We will need to utilize some structure of $K(\mathcal A)$ to facilitate arguments. 
The abstraction of this structure goes under the name of a _triangulated category_. 

**Definition**. Let $\mathcal T$ be an additive category equipped with 
an autoequivalence $[1] : \mathcal T \to \mathcal T$ and with a class of diagrams 
$$
    X \overset{\alpha}{\to} Y \overset{\beta}{\to} Z \overset{\gamma}{\to} X[1],
$$
called _triangles_. If the structure satisfies TR1)-TR4) below, then it 
is called a triangulated category. 

TR1) 
- For any $X$ 
$$ 
    X \overset{1_X}{\to} X \to 0 \to X[1]
$$ 
is a triangle. 
- For any $f: X \to Y$ there exists a triangle 
$$
    X \overset{f}{\to} Y \to Z \to X[1]
$$
- Given a triangle 
$$
    X \to Y \to Z \to X[1]
$$
and a commutative diagram 
    <center> 
    {% tikz iso_triangle %}
        \node (X) at (-4,2) {$X$};
        \node (Y) at (-2,2) {$Y$};
        \node (Z) at (0,2) {$Z$};
        \node (X1) at (2,2) {$X[1]$};
        \node (X') at (-4,0) {$X^\prime$};
        \node (Y') at (-2,0) {$Y^\prime$};
        \node (Z') at (0,0) {$Z^\prime$};
        \node (X1') at (2,0) {$X^\prime[1]$};
        \draw[->] (X) -- (Y);
        \draw[->] (Y) -- (Z);
        \draw[->] (Z) -- (X1);
        \draw[->] (X') -- (Y');
        \draw[->] (Y') -- (Z');
        \draw[->] (Z') -- (X1');
        \draw[->] (X) -- node[above, rotate=90] {$\sim$} node[right] {$f$} (X');
        \draw[->] (Y) -- node[above, rotate=90] {$\sim$} node[right] {$g$} (Y'); 
        \draw[->] (Z) -- node[above, rotate=90] {$\sim$} node[right] {$h$} (Z');
        \draw[->] (X1) -- node[above, rotate=90] {$\sim$} node[right] {$f[1]$} (X1');
    {% endtikz %}
    </center>
    where the vertical maps are isomorphisms, the diagram
    $$
        X^\prime \to Y^\prime \to Z^\prime \to X^\prime[1]
    $$
    is also a triangle.


TR2) If 
$$
    X \overset{\alpha}{\to} Y \overset{\beta}{\to} Z \overset{\gamma}{\to} X[1]
$$
is a triangle, then so are 
$$
    Y \overset{\beta}{\to} Z \overset{\gamma}{\to} X[1] \overset{\alpha[1]}{\to} Y[1]
$$
and
$$
    Z[-1] \overset{\gamma[-1]}{\to} X \overset{\alpha}{\to} Y \overset{\beta}{\to} Z 
$$

TR3) Given a commutative diagram 
<center> 
{% tikz tr3 %}
    \node (X) at (-4,2) {$X$};
    \node (Y) at (-2,2) {$Y$};
    \node (Z) at (0,2) {$Z$};
    \node (X1) at (2,2) {$X[1]$};
    \node (X') at (-4,0) {$X^\prime$};
    \node (Y') at (-2,0) {$Y^\prime$};
    \node (Z') at (0,0) {$Z^\prime$};
    \node (X1') at (2,0) {$X^\prime[1]$};
    \draw[->] (X) -- (Y);
    \draw[->] (Y) -- (Z);
    \draw[->] (Z) -- (X1);
    \draw[->] (X') -- (Y');
    \draw[->] (Y') -- (Z');
    \draw[->] (Z') -- (X1');
    \draw[->] (X) -- (X');
    \draw[->] (Y) -- (Y'); 
    \draw[->] (X1) -- (X1');
{% endtikz %}
</center>
with
$$ 
    X \to Y \to Z \to X[1]
$$ 
and 
$$ 
    X^\prime \to Y^\prime \to Z^\prime \to X^\prime[1]
$$ 
triangles, there exists a map $h: Z \to Z^\prime$ making the diagram 
<center> 
{% tikz tr3_completed %}
    \node (X) at (-4,2) {$X$};
    \node (Y) at (-2,2) {$Y$};
    \node (Z) at (0,2) {$Z$};
    \node (X1) at (2,2) {$X[1]$};
    \node (X') at (-4,0) {$X^\prime$};
    \node (Y') at (-2,0) {$Y^\prime$};
    \node (Z') at (0,0) {$Z^\prime$};
    \node (X1') at (2,0) {$X^\prime[1]$};
    \draw[->] (X) -- (Y);
    \draw[->] (Y) -- (Z);
    \draw[->] (Z) -- (X1);
    \draw[->] (X') -- (Y');
    \draw[->] (Y') -- (Z');
    \draw[->] (Z') -- (X1');
    \draw[->] (X) -- (X');
    \draw[->] (Y) -- (Y');
    \draw[->] (Z) -- node[left] {$h$} (Z'); 
    \draw[->] (X1) -- (X1');
{% endtikz %}
</center>
commute. 

TR4) (Octahedral Axiom) 
Given $\alpha: X \to Y$ and $\beta : Y \to Z$ we have a commutative diagram 
<center> 
{% tikz octahedral_axiom %}
    \node (Xa) at (-4,2) {$X$};
    \node (Y) at (-2,2) {$Y$};
    \node (Z') at (0,2) {$Z^\prime$};
    \node (X1a) at (2,2) {$X[1]$};
    \node (Xb) at (-4,0) {$X$};
    \node (Z) at (-2,0) {$Z$};
    \node (Y') at (0,0) {$Y^\prime$};
    \node (X1b) at (2,0) {$X[1]$};
    \node (02) at (-4,-2) {$0$};
    \node (X'a) at (-2,-2) {$X^\prime$};
    \node (X'b) at (0,-2) {$X^\prime$};
    \node (03) at (2,-2) {$0$};
    \node (X1) at (-4,-4) {$X[1]$};
    \node (Y1) at (-2,-4) {$Y[1]$};
    \node (Z1) at (0,-4) {$Z[1]$};
    \node (X2) at (2,-4) {$X[2]$};
    \draw[->] (Xa) -- node[above] {$\alpha$} (Y);
    \draw[->] (Y) -- (Z');
    \draw[->] (Z') -- (X1a);
    \draw[->] (Xa) -- node[left] {$=$} (Xb);
    \draw[->] (Y) -- node[left] {$\beta$} (Z); 
    \draw[->] (Z') -- (Y');
    \draw[->] (X1a) -- node[left] {$=$} (X1b);\
    \draw[->] (Xb) -- node[above] {$\beta \alpha$} (Z);
    \draw[->] (Z) -- (Y');
    \draw[->] (Y') -- (X1b);
    \draw[->] (Xb) -- (02);
    \draw[->] (Z) -- (X'a);
    \draw[->] (Y') -- (X'b);
    \draw[->] (X1b) -- (03);
    \draw[->] (02) -- (X'a);
    \draw[->] (X'a) -- node[above] {$=$} (X'b); 
    \draw[->] (X'b) -- (03);
    \draw[->] (02) -- (X1);
    \draw[->] (X'a) -- (Y1);
    \draw[->] (X'b) -- (Z1);
    \draw[->] (03) -- (X2);
    \draw[->] (X1) -- node[above] {$\alpha[1]$} (Y1);
    \draw[->] (Y1) -- (Z1);
    \draw[->] (Z1) -- (X2); 
{% endtikz %}
</center>
where all rows and columns are triangles.


## Basic consequences of the definition 

Triangles are automatically complexes. 

**Lemma**. Given a triangle 
$$
    X \overset{\alpha}{\to} Y \overset{\beta}{\to} Z \overset{\gamma}{\to} X[1]
$$
we have 
$$
\beta\alpha, \gamma\beta, \alpha[1]\gamma = 0.
$$

{% proof %}

From TR3), we can complete the diagram 

{% eqn triangle_is_complex %}
\begin{tikzcd}
X \arrow[r,"="] \arrow[d,"="] & X \arrow[r] \arrow[d,"\alpha"] & 0 \arrow[r] \arrow[d,dashed] & X[1] \arrow[d,"="] \\
X \arrow[r,"\alpha"] & Y \arrow[r,"\beta"] & Z \arrow[r] & X[1] 
\end{tikzcd}
{% endeqn %}

giving 
$$
\beta \alpha = 0.
$$ 
The other cases are handled similarly. 

{% endproof %}

**Definition**. A functor $H : \mathcal T \to \mathcal A$ from a triangulated category 
to an abelian category is _homological_ if for any triangle 
$$
    X \to Y \to Z \to X[1]
$$
the sequence 
$$
    HX \to HY \to HZ
$$
is exact. If a functor $H: \mathcal T^{op} \to \mathcal A$ is homological, 
we call it _cohomological_. 

The following is an immediate consequence. 

**Lemma**. If $H$ is homological, then there is a long exact sequence
$$
    \cdots \to H(Z[-1]) \to HX \to HY \to HZ \to H(X[1]) \to \cdots 
$$

{% proof %}
This is an immediate consequence of TR2). 
{% endproof %}

Representable functors are (co)homological.

**Lemma**. For any object $T$ of $\mathcal T$, the functor 
$\operatorname{Hom}\_{\mathcal T}(T,-)$ is homological and 
$\operatorname{Hom}\_{\mathcal T}(-,T)$ is cohomological.

{% proof %}

We treat the first case. Since any triangle is a complex, we already know that 
$$
    \cdots \to \operatorname{Hom}(T,X) \to \operatorname{Hom}(T,Y) \to \operatorname{Hom}(T,Z) \to \operatorname{Hom}(T,X[1]) \to \cdots
$$
is also a complex. Assume that $\beta f = 0$ for some $f: T \to Y$. Then, we can complete the diagram

{% eqn hom_is_homological %}
\begin{tikzcd}
T \arrow[d,"\exists g", swap, dashed] \arrow[r,"="] & T \arrow[r] \arrow[d,"f"] & 0 \arrow[r] \arrow[d] & T[1] \arrow[d,"="] \\
X \arrow[r] & Y \arrow[r] & Z \arrow[r] & X[1] 
\end{tikzcd}
{% endeqn %}

giving a $g$ with $\alpha g = f$. 

{% endproof %}

<!-- **Lemma**. If we have a diagram 
{% eqn two_of_three_iso_triangle %}
\begin{tikzcd}[row sep=huge]
X \arrow[d,"\sim"{sloped},"f"'] \arrow[r] & Y \arrow[d,"\sim"{sloped},"g"'] \arrow[r] & Z \arrow[d,"h"] \arrow[r] & X[1] \arrow[d,"\sim"{sloped},"f{[1]}"'] \\
X^\prime \arrow[r] & Y^\prime \arrow[r] & Z^\prime \arrow[r] & X^\prime[1]
\end{tikzcd}
{% endeqn %}
with the rows being triangles and with $f$ and $g$ being isomorphims, then $h$ is also an isomorphism. 

{% proof %}
For any $T$ we have a map of long exact sequences 
{% eqn 2_of_3_les %}
\begin{tikzcd}
\cdots \ar[r] & \operatorname{Hom}(T,X) \ar[r] \ar[d,"\sim"{sloped}] 
& \operatorname{Hom}(T,Y) \ar[r] \ar[d, "\sim"{sloped}] & 
\operatorname{Hom}(T,Z) \ar[r] \ar[d] & \operatorname{Hom}(T,X[1]) \ar[r] \ar[d,"\sim"{sloped}] & \cdots \\
\cdots \ar[r]  & \operatorname{Hom}(T,X^\prime) \ar[r]  & \operatorname{Hom}(T,Y^\prime) \ar[r]  & 
\operatorname{Hom}(T,Z^\prime) \ar[r]  & \operatorname{Hom}(T,X[1]^\prime) \ar[r]  & \cdots \\
\end{tikzcd}
{% endeqn %}
where two out of every three vertical maps are isomorphisms. Thus, the all must be so. 

Thus, $\operatorname{Hom}(-,Z) \cong \operatorname{Hom}(-,Z^\prime)$ and thus by Yoneda 
$$
    Z \cong Z^\prime
$$
{% endproof %} -->

**Definition**. A _candidate triangle_ is a diagram 
$$
    X \to Y \to Z \to X[1] 
$$
such that either 
$$
    \cdots \to \operatorname{Hom}(T,X) \to \operatorname{Hom}(T,Y) \to \operatorname{Hom}(T,Z) \to
    \operatorname{Hom}(T,X[1]) \to \cdots 
$$
is an exact sequence for all $T$ or 
$$
    \cdots \to \operatorname{Hom}(X[1],T) \to \operatorname{Hom}(Z,T) \to \operatorname{Hom}(Y,T) \to
    \operatorname{Hom}(X,T) \to \cdots 
$$
is an exact sequence for all $T$. 

A useful lemma in detecting triangles is the following. 

**Lemma**. Assume we have a map of candidate triangles
{% eqn candidate_triangle %}
\begin{tikzcd}
X^\prime \ar[r] \ar[d,"\sim"{sloped}] & Y^\prime \ar[r] \ar[d,"\sim"{sloped}] & Z^\prime \ar[r] \ar[d] & 
X^\prime[1] \ar[d,"\sim"{sloped}] \\
X \ar[r] & Y \ar[r] & Z \ar[r] & X[1] 
\end{tikzcd}
{% endeqn %}
with all maps labeled by $\sim$ isomorphisms. Then $Z \to Z^\prime$ is an isomorphism. 

In particular, if at least one of the candidate triangles is an actual triangle, so is the other. 

{% proof %}
We assume that applying $\operatorname{Hom}(T,-)$ to our candidate triangle yields an 
exact sequence. We apply $\operatorname{Hom}(T,-)$ to the whole diagram giving 
{% eqn candidate_triangle_les %}
\begin{tikzcd}
\cdots \ar[r] & \operatorname{Hom}(T,X^\prime) \ar[r] \ar[d,"\sim"{sloped}] & \operatorname{Hom}(T,Y^\prime) 
\ar[r] \ar[d,"\sim"{sloped}] & \operatorname{Hom}(T,Z^\prime) \ar[r] \ar[d] & \operatorname{Hom}(T,X^\prime[1]) 
\ar[r] \ar[d,"\sim"{sloped}] & \cdots \\
\cdots \ar[r] & \operatorname{Hom}(T,X) \ar[r]  & \operatorname{Hom}(T,Y) 
\ar[r]  & \operatorname{Hom}(T,Z) \ar[r]  & \operatorname{Hom}(T,X[1]) 
\ar[r]  & \cdots
\end{tikzcd}
{% endeqn %}
From the five lemma, we have an isomorphism 
$$
    \operatorname{Hom}(-,Z^\prime) \cong \operatorname{Hom}(-,Z)
$$
and hence by Yoneda $Z^\prime \cong Z$. Thus, we have an isomorphism between our triangle 
and candidate triangle. By TR1), the candidate triangle is triangle. 
{% endproof %}

Note that the previous lemma applies in the case both rows are triangles. In particular, it implies 
that the object $Z$ completing the triangle for $f: X \to Y$ is unique up to isomorphism. 

**Definition**. In a triangle 
$$
    X \overset{f}{\to} Y \to Z \to X[1]
$$
we call $Z$ the _cone_ of the morphism $f$. 

**Lemma**. A retract of a triangle is also a triangle. 

{% proof %}
Assume we have a diagram 
{% eqn retract_triangles %}
\begin{tikzcd}
adX^\prime \ar[d] \ar[dd,bend right=60, near end, swap, "1"] \ar[r,"f"] & Y^\prime \ar[r] \ar[d] \ar[dd,bend right=60, near end, swap, "1"] 
& Z^\prime \ar[r] \ar[d] \ar[dd,bend right=60, near end, swap, "1"] & X^\prime[1] \ar[d] \ar[dd,bend right=60, near end, swap, "1"] \\
X \ar[d] \ar[r] & Y \ar[r] \ar[d] & Z \ar[r] \ar[d] & X[1] \ar[d] \\
X^\prime \ar[r] & Y^\prime \ar[r] & Z^\prime \ar[r] & X^\prime[1] 
\end{tikzcd}
{% endeqn %}
Applying $\operatorname{Hom}(T,-)$ gives a retract of an exact sequence which is also exact. 

Now complete $f: X^\prime \to Y^\prime$ to a triangle:
$$
    X^\prime \to Y^\prime \to \bar{Z} \to X^\prime[1]
$$
We can complete the square 
{% eqn retract_square %}
\begin{tikzcd}
    X^\prime \ar[r] \ar[d] & Y^\prime \ar[r] \ar[d] & \bar{Z} \ar[r] \ar[d,dashed] 
    & X^\prime[1] \ar[d] \\
    X \ar[r] & Y \ar[r] & Z \ar[r] & X[1]
\end{tikzcd}
{% endeqn %}
and compose to get a map 
{% eqn retract_tri_map %}
\begin{tikzcd}
    X^\prime \ar[r] \ar[d,"="] & Y^\prime \ar[r] \ar[d,"="] 
    & \bar{Z} \ar[r] \ar[d] & X^\prime[1] \ar[d,"="] \\
    X^\prime \ar[r] & Y^\prime \ar[r] & Z^\prime \ar[r] & X^\prime[1]
\end{tikzcd}
{% endeqn %}
By the previous lemma, we have a triangle. 
{% endproof %}

We can play a similar strategy with other functorial constructions that preserve exact 
sequences. 

**Lemma**. Let 
$$
    X_i \to Y_i \to Z_i \to X_i[1]
$$
be triangles for $i \in I$. 
- If 
$$
    \bigoplus_I X_i \to \bigoplus_I Y_i \to \bigoplus_I Z_i \to \bigoplus_I X_i[1]
$$  
exists, it is a triangle. 
- If 
$$
    \prod_I X_i \to \prod_I Y_i \to \prod_I Z_i \to \prod_I X_i[1]
$$  
exists, it is a triangle.

{% proof %}
We treat $\bigoplus$ since $\prod$ follows analogously. Take a triangle 
$$
    \bigoplus X_i \to \bigoplus Y_i \to Z \to \bigoplus X_i[1]
$$
Note that the possibile ambiguity in writing $\bigoplus X_i[1]$ is fine 
since $[1]$, as an autoequivalence commutes with coproducts. 

For each $i$ we have a map of triangles 
{% eqn coprod_triangle %}
\begin{tikzcd}
    X_i \ar[r] \ar[d] & Y_i \ar[r] \ar[d] & Z_i \ar[r] \ar[d] & X_i[1] \ar[d] \\
    \bigoplus X_i \ar[r] & \bigoplus Y_i \ar[r] & Z \ar[r] & \bigoplus X_i[1]
\end{tikzcd}
{% endeqn %}
which gives a map 
{% eqn coprod_triangle_2 %}
\begin{tikzcd}
    \bigoplus X_i \ar[r] \ar[d] & \bigoplus Y_i \ar[r] \ar[d] & \bigoplus Z_i \ar[r] \ar[d] &
     \bigoplus X_i[1] \ar[d] \\
    \bigoplus X_i \ar[r] & \bigoplus Y_i \ar[r] & Z \ar[r] & \bigoplus X_i[1]
\end{tikzcd}
{% endeqn %}
The top row is a candidate triangle as products of exact sequences of abelian groups remain 
exact. Applying the previous lemma shows it is a triangle. 
{% endproof %}

Finally, we can detect isomorphisms using objects via triangles. 

**Lemma**. The map $f : X \to Y$ is an isomorphism in $\mathcal T$ if and only if 
$$
    X \overset{f}{\to} Y \to 0 \to X[1]
$$  
is a triangle. 

{% proof %}
For the forward direction assume $f$ is an isomorphism. Then we can construct a morphism of 
triangles 
{% eqn iso_cone_0 %}
\begin{tikzcd}
    X \ar[r,"f"] \ar[d,"f"] & Y \ar[r] \ar[d] & Z \ar[r] \ar[d] & X[1] \ar[d] \\
    Y \ar[r,"="] & Y \ar[r] & 0 \ar[r] & Y[1]
\end{tikzcd}
{% endeqn %}
showing $Z \cong 0$. 

In the other direction, we can apply $\operatorname{Hom}(T,-)$ and conclude that 
$$
    \operatorname{Hom}(-,f) : \operatorname{Hom}(-,X) \to \operatorname{Hom}(-,Y)
$$
is an isomorphism. Hence $f: X \to Y$ is also. 
{% endproof %}

## The homotopy category as a triangulated category 

For $K(\mathcal A)$ we already have the shift $[1]$. We just need to the collection of 
triangles. 

**Definition**. Given a chain map $\phi : A \to B$, the _cone_ of $\phi$ is the complex 
$$
    C(\phi)^i = A^{i+1} \oplus B^i, \ \delta^i_{C(\phi)} = \begin{pmatrix} -\delta_A^{i+1} & 0 \\
    \phi_{i+1} & \delta_B^i \end{pmatrix}
$$
There are chain maps given by inclusion
$$
    B \to C(\phi) 
$$
and by projection
$$
    C(\phi) \to A
$$

The triangles will be diagrams isomorphic to a triangle for the form 
$$
    A \overset{\phi}{\to} B \to C(\phi) \to A[1]
$$
for some $\phi : A \to B$. 

**Proposition**. The homotopy category $K(\mathcal A)$ with $[1]$ and these triangles is a 
triangulated category. 

One important fact to notice: this cone construction is a functorial. Given a square 
{% eqn square %}
\begin{tikzcd}
    A \ar[r,"f"] \ar[d,"\alpha"] & B \ar[d,"\beta"] \\
    A^\prime. \ar[r,"g"] & B^\prime
\end{tikzcd}
{% endeqn %}
we have a map of cones 
$$
    \begin{pmatrix} \alpha & 0 \\ 0 & \beta \end{pmatrix} : C(f) \to C(g)
$$

For a general triangulated category, this is not the case. 

Next, let's check (some of) the axioms in order of convenience. 

TR1) Clearly $C(1_A) \neq 0$ but we only need it to be null-homotopic. The map 
$$
    \begin{pmatrix} 0 & 1 \\ 0 & 0 \end{pmatrix} : A_{i+1} \oplus A_i \to A_i \oplus A_{i-1}
$$
provides the null-homotopy. 

The other two conditions here are automatic from the definition of the set of triangle: 
- Any map $\phi : A \to B$ can be completed to the triangle 
$$
    A \to B \to C(\phi) \to A[1]
$$
- Anything isomorphic to a triangle is itself a triangle as we declared that the set 
of triangles to be closed under isomorphism as part of the definition. 

TR3) We already mentioned the functoriality of the cone construction. Thus given a 
commutative square 
{% eqn tr2_cone_complex %}
\begin{tikzcd}
    A \ar[r,"f"] \ar[d] & B \ar[d] \\ 
    A^\prime \ar[r,"g"] & B^\prime
\end{tikzcd}
{% endeqn %}
we can complete it to a map of triangles 
{% eqn tr2_cone_complex_completed %}
\begin{tikzcd}
    A \ar[r] \ar[d] & B \ar[d] \ar[r] & C(f) \ar[r] \ar[d] & A[1] \\
    A^\prime \ar[r] & B^\prime \ar[r] & C(g) \ar[r] & B^\prime[1]
\end{tikzcd}
{% endeqn %}

TR2) This reduces to the claim that $C(C(\phi) \to A[1])$ is homotopic to $B[1]$ and that 
$C(B \to C(\phi))$ is homotopic to $A[1]$. We expand on the later claim. 

The projection defines a chain map 
$$
    \rho : C(B \to C(\phi)) \to A[1]. 
$$
The map in the other direction is 
$$
    \ell : \begin{pmatrix} \phi & 1 & 0 \end{pmatrix} A[1] \to C(B \to C(\phi)). 
$$

The composition $\rho \ell$ is $1_{A[1]}$. The other composition is homotopic to the identity via 
$$
    \begin{pmatrix} 0 & 0 & 1 \\ 0 & 0 & 0 \\ 0 & 0 & 0 \end{pmatrix} : C(B \to C(\phi)) \to C(B \to C(\phi))
$$

Checking the other claim boils down to producing such homotopies similar to some of the following observations 
that relate the abelian category structure of $Ch(\mathcal A)$ to cones. 

**Proposition**. 
- The sequence 
$$
    0 \to B \to C(\phi) \to A \to 0
$$
is an exact sequence of complexes. 
- Let $K = \ker \phi$ and $C = \operatorname{cok} \phi$. Then we can factor the map $K \to A$ as 
$$
    K \to C(\phi)[-1] \to A
$$  
and the map $B \to C$ as 
$$
    B \to C(\phi) \to C. 
$$
- If $\phi: A \hookrightarrow B$, then $C(\phi) \to C$ is a quasi-isomorphism. 
- If $\phi: A \twoheadrightarrow B$, the $K \to C(\phi)[-1]$ is a quasi-isomorphism. 

We leave the details to the reader. 

Finally, we ignore TR4) until we actually need it (as is tradition). 